BDDdummy_lemma_4.v
@@ -279,7 +279,7 @@ cut
                    (fst (BDDor_1 cfg memo (low cfg node1) node2 bound'))
                    (snd (snd (BDDor_1 cfg memo (low cfg node1) node2 bound')))
                    (high cfg node1) node2 bound'))))) /\
-  (Neqb (fst (snd (BDDor_1 cfg memo (low cfg node1) node2 bound')))
+  (N.eqb (fst (snd (BDDor_1 cfg memo (low cfg node1) node2 bound')))
      (fst
         (snd
            (BDDor_1 (fst (BDDor_1 cfg memo (low cfg node1) node2 bound'))
@@ -327,7 +327,7 @@ cut
           (BDDor_1 (fst (BDDor_1 cfg memo (low cfg node1) node2 bound'))
              (snd (snd (BDDor_1 cfg memo (low cfg node1) node2 bound')))
              (high cfg node1) node2 bound'))))) /\
-  (Neqb (fst (snd (BDDor_1 cfg memo (low cfg node1) node2 bound')))
+  (N.eqb (fst (snd (BDDor_1 cfg memo (low cfg node1) node2 bound')))
      (fst
         (snd
            (BDDor_1 (fst (BDDor_1 cfg memo (low cfg node1) node2 bound'))
@@ -526,7 +526,7 @@ rewrite
                    (snd (snd (BDDor_1 cfg memo (low cfg node1) node2 bound')))
                    (high cfg node1) node2 bound'))))) node1' node2')
  .
-elim (sumbool_of_bool (Neqb node1 node1' && Neqb node2 node2')); intro y2.
+elim (sumbool_of_bool (N.eqb node1 node1' && N.eqb node2 node2')); intro y2.
 rewrite y2.
 cut (node1 = node1').
 cut (node2 = node2').
@@ -726,10 +726,10 @@ rewrite
 exact H41.
 
 apply Neqb_complete.
-exact (proj2 (andb_prop (Neqb node1 node1') (Neqb node2 node2') y2)).
+exact (proj2 (andb_prop (N.eqb node1 node1') (N.eqb node2 node2') y2)).
 
 apply Neqb_complete.
-exact (proj1 (andb_prop (Neqb node1 node1') (Neqb node2 node2') y2)).
+exact (proj1 (andb_prop (N.eqb node1 node1') (N.eqb node2 node2') y2)).
 
 rewrite y2.
 intros.
